src/nextgen/nextgen_promises_model.v
@@ -11,7 +11,7 @@ From stdpp Require Import finite.
 From iris.algebra Require Import functions gmap agree excl csum max_prefix_list.
 From iris.algebra.lib Require Import mono_list.
 From iris.proofmode Require Import classes tactics.
-From iris.base_logic.lib Require Export iprop own invariants.
+From iris.base_logic.lib Require Export iprop own.
 From iris.prelude Require Import options.
 
 From iris_named_props Require Import named_props.
