src/nextgen/nextgen_promises_ng.v
@@ -1,25 +1,11 @@
 (* This file defines lemmas for cameras that do _not_ interact with the
  * [nextgen] modality and proves rules for these. *)
 
-From Equations Require Import Equations.
-From stdpp Require Import finite.
-
-From iris.algebra Require Import functions gmap agree excl csum max_prefix_list.
-From iris.algebra.lib Require Import mono_list.
 From iris.proofmode Require Import classes tactics.
-From iris.base_logic.lib Require Export iprop own invariants.
+From iris.base_logic.lib Require Export own.
 From iris.prelude Require Import options.
 
-From iris_named_props Require Import named_props.
-From nextgen Require Export nextgen_basic cmra_morphism_extra gen_single_shot gen_nc.
-
-From self Require Export hvec.
-From self.high Require Import increasing_map.
-From self.nextgen Require Export types omega generational_cmra transmap
-  promise nextgen_promises_model gen_ing.
-
-Import EqNotations. (* Get the [rew] notation. *)
-Import uPred.
+From self.nextgen Require Export nextgen_promises_model.
 
 (** Non-generational cameras. *)
 Class ngInG Σ (Ω : gGenCmras Σ) A := NgInG {
@@ -40,3 +26,4 @@ Section non_generational_resources.
     IntoNextgen _ _ := nextgen_ng_own γ a.
 
 End non_generational_resources.
+
